feat: RawAes KeyWrapping support (#169)
Support all edkWrapping types

AwsCryptographicMaterialProviders/dafny/AwsCryptographicMaterialProviders/src/Keyrings/RawAESKeyring.dfy
@@ -5,6 +5,8 @@ include "../Keyring.dfy"
 include "../Materials.dfy"
 include "../AlgorithmSuites.dfy"
 include "../Materials.dfy"
+include "../KeyWrapping/MaterialWrapping.dfy"
+include "../KeyWrapping/EdkWrapping.dfy"
 include "../CanonicalEncryptionContext.dfy"
 include "../../Model/AwsCryptographyMaterialProvidersTypes.dfy"
 
@@ -12,6 +14,7 @@ module RawAESKeyring {
   import opened StandardLibrary
   import opened UInt = StandardLibrary.UInt
   import opened String = StandardLibrary.String
+  import opened Actions
   import opened Wrappers
   import Types = AwsCryptographyMaterialProvidersTypes
   import Crypto = AwsCryptographyPrimitivesTypes
@@ -21,6 +24,8 @@ module RawAESKeyring {
   import opened AlgorithmSuites
   import UTF8
   import Seq
+  import MaterialWrapping
+  import EdkWrapping
 
   import Aws.Cryptography.Primitives
 
@@ -41,6 +46,7 @@ module RawAESKeyring {
       && cryptoPrimitives.Modifies <= Modifies
       && History !in cryptoPrimitives.Modifies
       && cryptoPrimitives.ValidState()
+      && |wrappingKey| == wrappingAlgorithm.keyLength as nat
     }
 
     const keyNamespace: UTF8.ValidUTF8Bytes
@@ -110,7 +116,7 @@ module RawAESKeyring {
     //= type=implication
     //# OnEncrypt MUST take [encryption materials](structures.md#encryption-
     //# materials) as input.
-    method  OnEncrypt'(input: Types.OnEncryptInput)
+    method {:vcs_split_on_every_assert} OnEncrypt'(input: Types.OnEncryptInput)
       returns (output: Result<Types.OnEncryptOutput, Types.Error>)
       requires ValidState()
       modifies Modifies - {History}
@@ -128,41 +134,28 @@ module RawAESKeyring {
       // EDK created using expected AAD
       ensures output.Success?
       ==>
+        // Verify AESEncrypt Input
         && CanonicalEncryptionContext.EncryptionContextToAAD(input.materials.encryptionContext).Success?
-        && |output.value.materials.encryptedDataKeys| == |input.materials.encryptedDataKeys| + 1
-        && |cryptoPrimitives.History.GenerateRandomBytes| == |old(cryptoPrimitives.History.GenerateRandomBytes)| + 2
-        && |cryptoPrimitives.History.AESEncrypt| == |old(cryptoPrimitives.History.AESEncrypt)| + 1
+        && 1 <= |cryptoPrimitives.History.GenerateRandomBytes|
         && Seq.Last(cryptoPrimitives.History.GenerateRandomBytes).output.Success?
-        && Seq.Last(Seq.DropLast(cryptoPrimitives.History.GenerateRandomBytes)).output.Success?
-        && Seq.Last(cryptoPrimitives.History.AESEncrypt).output.Success?
         && var iv :=  Seq.Last(cryptoPrimitives.History.GenerateRandomBytes).output.value;
+        && |iv| == wrappingAlgorithm.ivLength as nat
+        && 1 <= |cryptoPrimitives.History.AESEncrypt|
         && var AESEncryptInput := Seq.Last(cryptoPrimitives.History.AESEncrypt).input;
-        && var AESEncryptOutput := Seq.Last(cryptoPrimitives.History.AESEncrypt).output.value;
         && AESEncryptInput.encAlg == wrappingAlgorithm
         && AESEncryptInput.key == wrappingKey
         && AESEncryptInput.iv == iv
-        && AESEncryptInput.aad == CanonicalEncryptionContext.EncryptionContextToAAD(input.materials.encryptionContext).value 
+        && AESEncryptInput.aad == CanonicalEncryptionContext.EncryptionContextToAAD(input.materials.encryptionContext).value
+
+        // Verify AESEncrypt output
+        && |output.value.materials.encryptedDataKeys| == |input.materials.encryptedDataKeys| + 1
         && var edk := Seq.Last(output.value.materials.encryptedDataKeys);
-        && edk.keyProviderId == keyNamespace
-        && |iv| == wrappingAlgorithm.ivLength as int
+        && Seq.Last(cryptoPrimitives.History.AESEncrypt).output.Success?
+        && var AESEncryptOutput := Seq.Last(cryptoPrimitives.History.AESEncrypt).output.value;
         && edk.keyProviderInfo == SerializeProviderInfo(iv)
-        && edk.ciphertext == SerializeEDKCiphertext(AESEncryptOutput)
-
-      ensures
-        && output.Success?
-        && input.materials.plaintextDataKey.None?
-      ==>
-        && var plaintextDataKey := Seq.Last(Seq.DropLast(cryptoPrimitives.History.GenerateRandomBytes)).output.value;
-        && var AESEncryptInput := Seq.Last(cryptoPrimitives.History.AESEncrypt).input;
-        && AESEncryptInput.msg == plaintextDataKey
-        && output.value.materials.plaintextDataKey.value == plaintextDataKey
-
-      ensures
-        && output.Success?
-        && input.materials.plaintextDataKey.Some?
-      ==>
-        && Seq.Last(cryptoPrimitives.History.AESEncrypt).input.msg
-          == input.materials.plaintextDataKey.value
+        // Can not prove this at this time because if there is Wrapping involved
+        // then this will not be true.
+        // && edk.ciphertext == SerializeEDKCiphertext(AESEncryptOutput)
 
       //= aws-encryption-sdk-specification/framework/raw-aes-keyring.md#onencrypt
       //= type=implication
@@ -172,60 +165,31 @@ module RawAESKeyring {
     {
       var materials := input.materials;
       var suite := materials.algorithmSuite;
-      var aad :- CanonicalEncryptionContext.EncryptionContextToAAD(materials.encryptionContext);
 
-      // TODO add support
-      :- Need(materials.algorithmSuite.symmetricSignature.None?,
-        Types.AwsCryptographicMaterialProvidersException(
-          message := "Symmetric Signatures not yet implemented."));
-
-      // Random is a method, and transitions require both a key and encrypted data key
-      var randomKeyResult := cryptoPrimitives
-        .GenerateRandomBytes(Crypto.GenerateRandomBytesInput(length := GetEncryptKeyLength(suite)));
-      var k' :- randomKeyResult.MapFailure(e => Types.AwsCryptographyPrimitives(AwsCryptographyPrimitives := e));
-      var randomIvResult := cryptoPrimitives
-        .GenerateRandomBytes(Crypto.GenerateRandomBytesInput(length := wrappingAlgorithm.ivLength));
-      var iv :- randomIvResult.MapFailure(e => Types.AwsCryptographyPrimitives(AwsCryptographyPrimitives := e));
-      var providerInfo := SerializeProviderInfo(iv);
-
-      //= aws-encryption-sdk-specification/framework/raw-aes-keyring.md#onencrypt
-      //# If the [encryption materials](structures.md#encryption-materials) do
-      //# not contain a plaintext data key, OnEncrypt MUST generate a random
-      //# plaintext data key and set it on the [encryption materials]
-      //# (structures.md#encryption-materials).
-      var plaintextDataKey := if materials.plaintextDataKey.None? then
-        k'
-      else
-        materials.plaintextDataKey.value;
-
-      :- Need(|wrappingKey|== wrappingAlgorithm.keyLength as int,
-        Types.AwsCryptographicMaterialProvidersException( message := "Wrapping key length does not match algorithm"));
-
-      //= aws-encryption-sdk-specification/framework/raw-aes-keyring.md#onencrypt
-      //# The keyring MUST encrypt the plaintext data key in the [encryption
-      //# materials](structures.md#encryption-materials) using AES-GCM.
-      var aesEncryptResult := cryptoPrimitives
-        .AESEncrypt(
-          Crypto.AESEncryptInput(
-            encAlg := wrappingAlgorithm,
-            iv := iv ,
-            key := wrappingKey ,
-            msg := plaintextDataKey ,
-            aad := aad 
-          )
+      var wrap := new AesWrapKeyMaterial(
+        wrappingKey,
+        wrappingAlgorithm,
+        cryptoPrimitives
       );
-      var encryptResult :- aesEncryptResult.MapFailure(e => Types.AwsCryptographyPrimitives(AwsCryptographyPrimitives := e));
-      var encryptedKey := SerializeEDKCiphertext(encryptResult);
+      var generateAndWrap := new AesGenerateAndWrapKeyMaterial(wrap);
 
-      :- Need(HasUint16Len(providerInfo),
-        Types.AwsCryptographicMaterialProvidersException( message := "Serialized provider info too long."));
-      :- Need(HasUint16Len(encryptedKey),
-        Types.AwsCryptographicMaterialProvidersException( message := "Encrypted data key too long."));
+      var wrapOutput :- EdkWrapping.WrapEdkMaterial<AesWrapInfo>(
+        encryptionMaterials := materials,
+        wrap := wrap,
+        generateAndWrap := generateAndWrap
+      );
+
+      var symmetricSigningKeyList :=
+        if wrapOutput.symmetricSigningKey.Some? then
+          Some([wrapOutput.symmetricSigningKey.value])
+        else
+          None;
 
       var edk: Types.EncryptedDataKey := Types.EncryptedDataKey(
         keyProviderId := keyNamespace,
-        keyProviderInfo := providerInfo,
-        ciphertext := encryptedKey);
+        keyProviderInfo := SerializeProviderInfo(wrapOutput.wrapInfo.iv),
+        ciphertext := wrapOutput.wrappedMaterial
+      );
 
       //= aws-encryption-sdk-specification/framework/raw-aes-keyring.md#onencrypt
       //# The keyring MUST append the constructed encrypted data key to the
@@ -235,12 +199,27 @@ module RawAESKeyring {
       //= aws-encryption-sdk-specification/framework/raw-aes-keyring.md#onencrypt
       //# OnEncrypt MUST output the modified [encryption materials]
       //# (structures.md#encryption-materials).
-      var nextMaterials :- if materials.plaintextDataKey.None? then
-        Materials.EncryptionMaterialAddDataKey(materials, plaintextDataKey, [edk], None)
-      else
-        Materials.EncryptionMaterialAddEncryptedDataKeys(materials, [edk], None);
-      var result := Types.OnEncryptOutput(materials := nextMaterials);
-      return Success(result);
+      if (wrapOutput.GenerateAndWrapEdkMaterialOutput?) {
+        var result :- Materials.EncryptionMaterialAddDataKey(
+          materials,
+          wrapOutput.plaintextDataKey,
+          [edk],
+          symmetricSigningKeyList
+        );
+        return Success(Types.OnEncryptOutput(
+          materials := result
+        ));
+      } else if (wrapOutput.WrapOnlyEdkMaterialOutput?) {
+        // wrapped existing pdk. Add new edk to materials.
+        var result :- Materials.EncryptionMaterialAddEncryptedDataKeys(
+          materials,
+          [edk],
+          symmetricSigningKeyList
+        );
+        return Success(Types.OnEncryptOutput(
+          materials := result
+        ));
+      }
     }
 
     predicate OnDecryptEnsuresPublicly(input: Types.OnDecryptInput, output: Result<Types.OnDecryptOutput, Types.Error>){true}
@@ -264,7 +243,6 @@ module RawAESKeyring {
           input.materials,
           output.value.materials
         )
-      // TODO: ensure non-None when input edk list has edk with valid provider info
 
       // Plaintext decrypted using expected AAD
       ensures
@@ -280,7 +258,7 @@ module RawAESKeyring {
         && AESDecryptRequest.key == wrappingKey
         && (exists edk
           | edk in input.encryptedDataKeys
-          :: 
+          ::
             && ValidProviderInfo(edk.keyProviderInfo)
             && wrappingAlgorithm.tagLength as nat <= |edk.ciphertext|
             && var encryptionOutput := DeserializeEDKCiphertext(
@@ -327,32 +305,40 @@ module RawAESKeyring {
       {
         if ShouldDecryptEDK(input.encryptedDataKeys[i]) {
 
-          var iv := GetIvFromProvInfo(input.encryptedDataKeys[i].keyProviderInfo);
-          var encryptionOutput := DeserializeEDKCiphertext(
-            input.encryptedDataKeys[i].ciphertext,
-            wrappingAlgorithm.tagLength as nat
+          var edk := input.encryptedDataKeys[i];
+          var iv := GetIvFromProvInfo(edk.keyProviderInfo);
+
+          var unwrap := new AesUnwrapKeyMaterial(
+            wrappingKey,
+            wrappingAlgorithm,
+            iv,
+            cryptoPrimitives
+          );
+          var unwrapOutput := EdkWrapping.UnwrapEdkMaterial(
+            edk.ciphertext,
+            materials,
+            unwrap
           );
 
-          var ptKeyRes := this.Decrypt(iv, encryptionOutput, input.materials.encryptionContext);
-          if ptKeyRes.Success?
+          if unwrapOutput.Success?
           {
-            :- Need(
-              GetEncryptKeyLength(materials.algorithmSuite) as nat == |ptKeyRes.Extract()|,
-              // this should never happen
-              Types.AwsCryptographicMaterialProvidersException( message := "Plaintext Data Key is not the expected length"));
             //= aws-encryption-sdk-specification/framework/raw-aes-keyring.md#ondecrypt
             //# If a decryption succeeds, this keyring MUST add the resulting
             //# plaintext data key to the decryption materials and return the
             //# modified materials.
-            var result :- Materials.DecryptionMaterialsAddDataKey(materials, ptKeyRes.Extract(), None);
+            var result :- Materials.DecryptionMaterialsAddDataKey(
+              materials,
+              unwrapOutput.value.plaintextDataKey,
+              unwrapOutput.value.symmetricSigningKey
+            );
             var value := Types.OnDecryptOutput(materials := result);
             return Success(value);
           } else {
-            errors := errors + [ptKeyRes.error];
+            errors := errors + [unwrapOutput.error];
           }
         } else {
           errors := errors + [
-            Types.AwsCryptographicMaterialProvidersException( 
+            Types.AwsCryptographicMaterialProvidersException(
               message :="EncrypedDataKey "
               + Base10Int2String(i)
               + " did not match AESKeyring. " )
@@ -363,51 +349,6 @@ module RawAESKeyring {
       //# If no decryption succeeds, the keyring MUST fail and MUST NOT modify
       //# the [decryption materials](structures.md#decryption-materials).
       return Failure(Types.CollectionOfErrors(list := errors));
-    }
-
-    //TODO This needs to be a private method
-    method Decrypt(
-      iv: seq<uint8>,
-      encryptionOutput: Crypto.AESEncryptOutput,
-      encryptionContext: Types.EncryptionContext
-    ) returns (res: Result<seq<uint8>, Types.Error>)
-      requires |encryptionOutput.authTag| == wrappingAlgorithm.tagLength as int
-      requires |wrappingKey| == wrappingAlgorithm.keyLength as int
-      requires ValidState()
-      modifies Modifies - {History}
-      ensures ValidState()
-      ensures unchanged(History)
-      ensures
-        res.Success?
-      ==>
-        && |old(cryptoPrimitives.History.AESDecrypt)| + 1 == |cryptoPrimitives.History.AESDecrypt|
-        && Seq.Last(cryptoPrimitives.History.AESDecrypt).output.Success?
-        && CanonicalEncryptionContext.EncryptionContextToAAD(encryptionContext).Success?
-        && var AESDecryptRequest := Seq.Last(cryptoPrimitives.History.AESDecrypt).input;
-        && AESDecryptRequest.encAlg == wrappingAlgorithm
-        && AESDecryptRequest.key == wrappingKey
-        && AESDecryptRequest.cipherTxt == encryptionOutput.cipherText
-        && AESDecryptRequest.authTag == encryptionOutput.authTag
-        && AESDecryptRequest.iv == iv
-        && AESDecryptRequest.aad == CanonicalEncryptionContext.EncryptionContextToAAD(encryptionContext).value
-        && res.value
-          == Seq.Last(cryptoPrimitives.History.AESDecrypt).output.value;
-    {
-      :- Need(|iv| == wrappingAlgorithm.ivLength as int, Types.AwsCryptographicMaterialProvidersException( message := ""));
-      var aad :- CanonicalEncryptionContext.EncryptionContextToAAD(encryptionContext);
-      var maybePtKey := cryptoPrimitives
-        .AESDecrypt(
-          Crypto.AESDecryptInput(
-            encAlg := wrappingAlgorithm,
-            key := wrappingKey,
-            cipherTxt := encryptionOutput.cipherText,
-            authTag := encryptionOutput.authTag,
-            iv := iv,
-            aad := aad
-          )
-      );
-      var ptKey :- maybePtKey.MapFailure(e => Types.AwsCryptographyPrimitives(AwsCryptographyPrimitives := e));
-      return Success(ptKey);
     }
 
     function method SerializeProviderInfo(iv: seq<uint8>): seq<uint8>
@@ -424,7 +365,6 @@ module RawAESKeyring {
       // The key provider ID of the encrypted data key has a value equal to this keyring's key namespace.
       && edk.keyProviderId == keyNamespace
       && ValidProviderInfo(edk.keyProviderInfo)
-      && wrappingAlgorithm.tagLength as int <= |edk.ciphertext|
     }
 
     // TODO #68: prove providerInfo serializes/deserializes correctly
@@ -481,5 +421,317 @@ module RawAESKeyring {
     requires tagLen <= |ciphertext|
     ensures SerializeEDKCiphertext(DeserializeEDKCiphertext(ciphertext, tagLen)) == ciphertext
   {}
+
+  datatype AesUnwrapInfo = AesUnwrapInfo()
+  datatype AesWrapInfo = AesWrapInfo( iv: seq<uint8> )
+
+  class AesGenerateAndWrapKeyMaterial
+    extends MaterialWrapping.GenerateAndWrapMaterial<AesWrapInfo>
+  {
+    const wrap: AesWrapKeyMaterial
+
+    constructor(
+      wrap: AesWrapKeyMaterial
+    )
+      requires wrap.Invariant()
+      ensures this.wrap == wrap
+      ensures Invariant()
+    {
+      this.wrap := wrap;
+      Modifies := wrap.Modifies;
+    }
+
+    predicate Invariant()
+      reads Modifies
+      decreases Modifies
+    {
+      && Modifies == wrap.Modifies
+      && wrap.Invariant()
+    }
+
+    predicate Ensures(
+      input: MaterialWrapping.GenerateAndWrapInput,
+      res: Result<MaterialWrapping.GenerateAndWrapOutput<AesWrapInfo>, Types.Error>,
+      attemptsState: seq<ActionInvoke<MaterialWrapping.GenerateAndWrapInput, Result<MaterialWrapping.GenerateAndWrapOutput<AesWrapInfo>, Types.Error>>>
+    )
+      reads Modifies
+      decreases Modifies
+    {
+        res.Success?
+      ==>
+        && Invariant()
+        && 2 <= |wrap.cryptoPrimitives.History.GenerateRandomBytes|
+        && Seq.Last(Seq.DropLast(wrap.cryptoPrimitives.History.GenerateRandomBytes)).output.Success?
+        && var plaintextMaterial := Seq.Last(Seq.DropLast(wrap.cryptoPrimitives.History.GenerateRandomBytes)).output.value;
+        && res.value.plaintextMaterial == plaintextMaterial
+        && wrap.Ensures(
+          MaterialWrapping.WrapInput(
+            plaintextMaterial := plaintextMaterial,
+            algorithmSuite := input.algorithmSuite,
+            encryptionContext := input.encryptionContext
+          ),
+          Success(MaterialWrapping.WrapOutput(
+            wrappedMaterial := res.value.wrappedMaterial,
+            wrapInfo := res.value.wrapInfo
+          )),
+          []
+        )
+      && |res.value.plaintextMaterial| == AlgorithmSuites.GetEncryptKeyLength(input.algorithmSuite) as nat
+    }
+
+    method Invoke(
+      input: MaterialWrapping.GenerateAndWrapInput,
+      ghost attemptsState: seq<ActionInvoke<MaterialWrapping.GenerateAndWrapInput, Result<MaterialWrapping.GenerateAndWrapOutput<AesWrapInfo>, Types.Error>>>
+    ) returns (res: Result<MaterialWrapping.GenerateAndWrapOutput<AesWrapInfo>, Types.Error>)
+      requires Invariant()
+      modifies Modifies
+      decreases Modifies
+      ensures Invariant()
+      ensures Ensures(input, res, attemptsState)
+    {
+
+      var generateBytesResult := wrap.cryptoPrimitives.GenerateRandomBytes(
+        Crypto.GenerateRandomBytesInput(
+          length := AlgorithmSuites.GetEncryptKeyLength(input.algorithmSuite)
+        )
+      );
+      var plaintextMaterial :- generateBytesResult.MapFailure(
+        e => Types.AwsCryptographyPrimitives(AwsCryptographyPrimitives := e)
+      );
+
+      ghost var oldGenerateRandomBytes := wrap.cryptoPrimitives.History.GenerateRandomBytes;
+
+      var wrapOutput: MaterialWrapping.WrapOutput<AesWrapInfo> :- wrap.Invoke(
+        MaterialWrapping.WrapInput(
+          plaintextMaterial := plaintextMaterial,
+          algorithmSuite := input.algorithmSuite,
+          encryptionContext := input.encryptionContext
+        ), []);
+
+      res := Success(MaterialWrapping.GenerateAndWrapOutput(
+        plaintextMaterial := plaintextMaterial,
+        wrappedMaterial := wrapOutput.wrappedMaterial,
+        wrapInfo := wrapOutput.wrapInfo
+      ));
+
+      // This surgery is unfortunate, but required to forward
+      // the history and prove that we used it correctly.
+      wrap.cryptoPrimitives.History.GenerateRandomBytes := oldGenerateRandomBytes + [Seq.Last(wrap.cryptoPrimitives.History.GenerateRandomBytes)];
+
+    }
+
+  }
+
+  class AesWrapKeyMaterial
+    extends MaterialWrapping.WrapMaterial<AesWrapInfo>
+  {
+    const wrappingKey: seq<uint8>
+    const wrappingAlgorithm: Crypto.AES_GCM
+    const cryptoPrimitives: Primitives.AtomicPrimitivesClient
+
+    constructor(
+      wrappingKey: seq<uint8>,
+      wrappingAlgorithm: Crypto.AES_GCM,
+      cryptoPrimitives: Primitives.AtomicPrimitivesClient
+    )
+      requires cryptoPrimitives.ValidState()
+      ensures
+        && this.wrappingKey == wrappingKey
+        && this.wrappingAlgorithm == wrappingAlgorithm
+        && this.cryptoPrimitives == cryptoPrimitives
+      ensures Invariant()
+    {
+      this.wrappingKey := wrappingKey;
+      this.wrappingAlgorithm := wrappingAlgorithm;
+      this.cryptoPrimitives := cryptoPrimitives;
+      Modifies := cryptoPrimitives.Modifies;
+    }
+
+    predicate Invariant()
+      reads Modifies
+      decreases Modifies
+    {
+      && cryptoPrimitives.ValidState()
+      && Modifies == cryptoPrimitives.Modifies
+    }
+
+    predicate Ensures(
+      input: MaterialWrapping.WrapInput,
+      res: Result<MaterialWrapping.WrapOutput<AesWrapInfo>, Types.Error>,
+      attemptsState: seq<ActionInvoke<MaterialWrapping.WrapInput, Result<MaterialWrapping.WrapOutput<AesWrapInfo>, Types.Error>>>
+    )
+      reads Modifies
+      decreases Modifies
+    {
+      && (res.Success?
+      ==>
+        && Invariant()
+        && CanonicalEncryptionContext.EncryptionContextToAAD(input.encryptionContext).Success?
+        && 0 < |cryptoPrimitives.History.GenerateRandomBytes|
+        && 0 < |cryptoPrimitives.History.AESEncrypt|
+        && Seq.Last(cryptoPrimitives.History.GenerateRandomBytes).output.Success?
+        && Seq.Last(cryptoPrimitives.History.AESEncrypt).output.Success?
+        && var iv :=  Seq.Last(cryptoPrimitives.History.GenerateRandomBytes).output.value;
+        && var AESEncryptInput := Seq.Last(cryptoPrimitives.History.AESEncrypt).input;
+        && var AESEncryptOutput := Seq.Last(cryptoPrimitives.History.AESEncrypt).output.value;
+        && |iv| == wrappingAlgorithm.ivLength as nat
+        && AESEncryptInput.encAlg == wrappingAlgorithm
+        && AESEncryptInput.key == wrappingKey
+        && AESEncryptInput.iv == iv
+        && AESEncryptInput.aad == CanonicalEncryptionContext.EncryptionContextToAAD(input.encryptionContext).value
+        && res.value.wrappedMaterial == SerializeEDKCiphertext(AESEncryptOutput)
+        && res.value.wrapInfo.iv == iv
+      )
+    }
+
+    method Invoke(
+      input: MaterialWrapping.WrapInput,
+      ghost attemptsState: seq<ActionInvoke<MaterialWrapping.WrapInput, Result<MaterialWrapping.WrapOutput<AesWrapInfo>, Types.Error>>>
+    ) returns (res: Result<MaterialWrapping.WrapOutput<AesWrapInfo>, Types.Error>)
+      requires Invariant()
+      modifies Modifies
+      decreases Modifies
+      ensures Invariant()
+      ensures Ensures(input, res, attemptsState)
+    {
+
+      var aad :- CanonicalEncryptionContext.EncryptionContextToAAD(input.encryptionContext);
+      var randomIvResult := cryptoPrimitives
+        .GenerateRandomBytes(Crypto.GenerateRandomBytesInput(length := wrappingAlgorithm.ivLength));
+      var iv :- randomIvResult.MapFailure(e => Types.AwsCryptographyPrimitives(AwsCryptographyPrimitives := e));
+      //= aws-encryption-sdk-specification/framework/raw-aes-keyring.md#onencrypt
+      //# The keyring MUST encrypt the plaintext data key in the [encryption
+      //# materials](structures.md#encryption-materials) using AES-GCM.
+      var aesEncryptResult := cryptoPrimitives
+        .AESEncrypt(
+          Crypto.AESEncryptInput(
+            encAlg := wrappingAlgorithm,
+            iv := iv ,
+            key := wrappingKey ,
+            msg := input.plaintextMaterial,
+            aad := aad
+          )
+      );
+      var wrappedMaterialResult :- aesEncryptResult.MapFailure(e => Types.AwsCryptographyPrimitives(AwsCryptographyPrimitives := e));
+      var wrappedMaterial := SerializeEDKCiphertext(wrappedMaterialResult);
+
+      return Success(MaterialWrapping.WrapOutput(
+        wrappedMaterial := wrappedMaterial,
+        wrapInfo := AesWrapInfo(iv)
+      ));
+    }
+  }
+
+  class AesUnwrapKeyMaterial
+    extends MaterialWrapping.UnwrapMaterial<AesUnwrapInfo>
+  {
+    const wrappingKey: seq<uint8>
+    const wrappingAlgorithm: Crypto.AES_GCM
+    const iv: seq<uint8>
+    const cryptoPrimitives: Primitives.AtomicPrimitivesClient
+
+    constructor(
+      wrappingKey: seq<uint8>,
+      wrappingAlgorithm: Crypto.AES_GCM,
+      iv: seq<uint8>,
+      cryptoPrimitives: Primitives.AtomicPrimitivesClient
+    )
+      requires cryptoPrimitives.ValidState()
+      requires |iv| == wrappingAlgorithm.ivLength as nat
+      ensures
+        && this.wrappingKey == wrappingKey
+        && this.iv == iv
+        && this.wrappingAlgorithm == wrappingAlgorithm
+        && this.cryptoPrimitives == cryptoPrimitives
+      ensures Invariant()
+    {
+      this.wrappingKey := wrappingKey;
+      this.iv := iv;
+      this.wrappingAlgorithm := wrappingAlgorithm;
+      this.cryptoPrimitives := cryptoPrimitives;
+      Modifies := cryptoPrimitives.Modifies;
+    }
+
+    predicate Invariant()
+      reads Modifies
+      decreases Modifies
+    {
+      && cryptoPrimitives.ValidState()
+      && Modifies == cryptoPrimitives.Modifies
+      && |iv| == wrappingAlgorithm.ivLength as nat
+    }
+
+    predicate Ensures(
+      input: MaterialWrapping.UnwrapInput,
+      res: Result<MaterialWrapping.UnwrapOutput<AesUnwrapInfo>, Types.Error>,
+      attemptsState: seq<ActionInvoke<MaterialWrapping.UnwrapInput, Result<MaterialWrapping.UnwrapOutput<AesUnwrapInfo>, Types.Error>>>
+    )
+      reads Modifies
+      decreases Modifies
+    {
+        res.Success?
+      ==>
+        && Invariant()
+        && |res.value.unwrappedMaterial| == AlgorithmSuites.GetEncryptKeyLength(input.algorithmSuite) as nat
+        && CanonicalEncryptionContext.EncryptionContextToAAD(input.encryptionContext).Success?
+        && wrappingAlgorithm.tagLength as nat <= |input.wrappedMaterial|
+        && var encryptionOutput := DeserializeEDKCiphertext(
+            input.wrappedMaterial,
+            wrappingAlgorithm.tagLength as nat
+          );
+        && 0 < |cryptoPrimitives.History.AESDecrypt|
+        && Seq.Last(cryptoPrimitives.History.AESDecrypt).output.Success?
+        && var AESDecryptInput := Seq.Last(cryptoPrimitives.History.AESDecrypt).input;
+        && AESDecryptInput.encAlg == wrappingAlgorithm
+        && AESDecryptInput.key == wrappingKey
+        && AESDecryptInput.cipherTxt == encryptionOutput.cipherText
+        && AESDecryptInput.authTag == encryptionOutput.authTag
+        && AESDecryptInput.iv == iv
+        && AESDecryptInput.aad == CanonicalEncryptionContext.EncryptionContextToAAD(input.encryptionContext).value
+        && res.value.unwrappedMaterial
+          == Seq.Last(cryptoPrimitives.History.AESDecrypt).output.value
+    }
+
+    method Invoke(
+      input: MaterialWrapping.UnwrapInput,
+      ghost attemptsState: seq<ActionInvoke<MaterialWrapping.UnwrapInput, Result<MaterialWrapping.UnwrapOutput<AesUnwrapInfo>, Types.Error>>>
+    ) returns (res: Result<MaterialWrapping.UnwrapOutput<AesUnwrapInfo>, Types.Error>)
+      requires Invariant()
+      modifies Modifies
+      decreases Modifies
+      ensures Invariant()
+      ensures Ensures(input, res, attemptsState)
+    {
+      var aad :- CanonicalEncryptionContext.EncryptionContextToAAD(input.encryptionContext);
+      :- Need(
+        wrappingAlgorithm.tagLength as nat <= |input.wrappedMaterial|,
+        Types.AwsCryptographicMaterialProvidersException( message := "Insufficient data to decrypt."));
+      var encryptionOutput := DeserializeEDKCiphertext(
+        input.wrappedMaterial,
+        wrappingAlgorithm.tagLength as nat
+      );
+      var maybePtKey := cryptoPrimitives
+        .AESDecrypt(
+          Crypto.AESDecryptInput(
+            encAlg := wrappingAlgorithm,
+            key := wrappingKey,
+            cipherTxt := encryptionOutput.cipherText,
+            authTag := encryptionOutput.authTag,
+            iv := iv,
+            aad := aad
+          )
+      );
+      var ptKey :- maybePtKey.MapFailure(e => Types.AwsCryptographyPrimitives(AwsCryptographyPrimitives := e));
+      :- Need(
+        GetEncryptKeyLength(input.algorithmSuite) as nat == |ptKey|,
+        Types.AwsCryptographicMaterialProvidersException( message := "Plaintext Data Key is not the expected length"));
+
+      return Success(MaterialWrapping.UnwrapOutput(
+        unwrappedMaterial := ptKey,
+        unwrapInfo := AesUnwrapInfo
+      ));
+
+    }
+  }
 
 }
